examples/containers/theories/SequenceProofs/Applicative_liftA2.v
@@ -1,5 +1,5 @@
 From Coq Require Import
-  Lia Morphisms.
+  Lia Morphisms Program.Tactics.
 Require Import GHC.Base.
 Require Import Proofs.GHC.Base.
 Import GHC.Base.Notations.
@@ -15,9 +15,127 @@ Require Import SequenceProofs.ValidityFunction.
 Require Import SequenceProofs.Applicative_Internal.
 Require Import SequenceProofs.Applicative_aptyMiddle.
 
+Local Open Scope Z_scope.
+
 Opaque aptyMiddle.
 
 Ltac auto_valid := fold_classes; auto_valid_.
+
+Definition valid_with_size {A} `{Sized A} `{Validity A} (n : Int) : A -> Prop :=
+  fun a => valid a /\ size a = n.
+
+Definition midsize {A} `{Sized A} (t : Rigid A) : Int :=
+  match t with
+  | Mk_Rigid _ _ m _ => size m
+  end.
+
+Lemma FMultSizedValid_ElemToNode2 {A B C} `{Sized B} `{Validity B} `{Sized C} `{Validity C}
+    (s : Int) (map23 : A -> B -> C)
+    (pr sf : Digit23 B)
+  : s = size pr + size sf ->
+    (forall a, FSizedValid (map23 a)) ->
+    valid pr -> valid sf ->
+    FMultSizedValid s
+      (fun '(Mk_Elem f) =>
+         Node2 (size pr + size sf) (fmap (map23 f) pr) (fmap (map23 f) sf)).
+Proof.
+  split; intros []; cbn; fold_classes.
+  - subst s; cbn; clear; lia.
+  - intros _.
+    split.
+    + rewrite 2 size_fmap__Node; auto.
+    + split; apply valid_fmap__Node; auto.
+Qed.
+
+Lemma FMultSizedValid_ElemToNode3 {A B C} `{Sized B} `{Validity B} `{Sized C} `{Validity C}
+    (s : Int) (map23 : A -> B -> C)
+    (pr sf n : Digit23 B)
+  : s = size pr + size n + size sf ->
+    (forall a, FSizedValid (map23 a)) ->
+    valid pr -> valid sf -> valid n ->
+    FMultSizedValid s
+      (fun '(Mk_Elem f) =>
+         Node3 (size pr + size n + size sf)
+           (fmap (map23 f) pr)
+           (fmap (map23 f) n)
+           (fmap (map23 f) sf)).
+Proof.
+  split; intros []; cbn; fold_classes.
+  * subst s; cbn; clear; lia.
+  * intros _.
+    split; [ | auto_valid ].
+    rewrite 3 size_fmap__Node; auto.
+Qed.
+
+Section aptyMiddle.
+
+Context {B C A : Type}
+  `{SizedB : Sized B} `{ValidityB : Validity B} `{SizedC : Sized C} `{ValidityC : Validity C}
+  (firstf : B -> C) (lastf : B -> C) (map23 : A -> B -> C)
+  (ta : FingerTree (Elem A)) (tb : Rigid B)
+  (Hfirstf : FSizedValid firstf)
+  (Hlastf : FSizedValid lastf)
+  (Hmap23 : forall a, FSizedValid (map23 a))
+  (Hta : valid ta)
+  (Htb : valid tb).
+
+Opaque aptyMiddle.
+
+Theorem valid_with_size_aptyMiddle
+  : valid_with_size
+      (midsize tb + size tb + size ta * size tb)
+      (aptyMiddle firstf lastf map23 ta tb).
+Proof.
+  revert_until tb. revert SizedB ValidityB SizedC ValidityC.
+  apply aptyMiddle_ind; clear; intros B C A firstf lastf map23 ta tb IH; intros.
+  rewrite unfold_aptyMiddle.
+  destruct tb as [ s pr m sf ]; decompose_conj Htb.
+  destruct m as [ | | sm prm mm sfm ].
+  + red; cbn.
+    pose proof (FMultSizedValid_ElemToNode2 s map23 pr sf) as MMF.
+    prove_assumptions_of MMF; try solve [ auto | subst; clear; cbn; lia ].
+    split.
+    * auto_valid.
+      apply valid_mapMulFT; auto.
+    * fold_classes. rewrite 2 size_fmap__Node; auto_valid.
+      rewrite size_mapMulFT; auto.
+      subst; clear; cbn; lia.
+  + red; cbn.
+    pose proof (FMultSizedValid_ElemToNode3 s map23 pr sf) as MMF.
+    prove_assumptions_of MMF; auto.
+    split.
+    * auto_valid.
+      apply valid_mapMulFT; auto.
+    * fold_classes. rewrite !size_fmap__Node; auto_valid.
+      rewrite size_mapMulFT; auto.
+      subst; clear; cbn; lia.
+  + match goal with
+    | [ H : valid__Thin (DeepTh _ _ _ _) |- _ ] => decompose_conj H
+    end.
+    specialize (IH _ _ _ (fmap firstf) (fmap lastf) (fmap GHC.Base.∘ map23) ta (Mk_Rigid s (squashL pr prm) mm (squashR sfm sf)) eq_refl _ _ _ _).
+    prove_assumptions_of IH; auto_valid.
+      { cbn. fold_classes.
+        split.
+        { rewrite size_squashL, size_squashR.
+          subst; cbn; lia. }
+        { auto using @valid_squashL, @valid_squashR. } }
+    destruct IH as [ IHvalid IHsize ].
+    split.
+    * cbn. auto_valid.
+      { rewrite IHsize. cbn. fold_classes. rewrite 2 size_digit12ToDigit by auto.
+        subst s sm; cbn; lia.  }
+    * cbn. lia.
+Qed.
+
+Lemma size_aptyMiddle
+  : size (aptyMiddle firstf lastf map23 ta tb) =
+    midsize tb + size tb + size ta * size tb.
+Proof. apply valid_with_size_aptyMiddle. Qed.
+
+Lemma valid_aptyMiddle : valid (aptyMiddle firstf lastf map23 ta tb).
+Proof. apply valid_with_size_aptyMiddle. Qed.
+
+End aptyMiddle.
 
 Section liftA2.
 
@@ -30,10 +148,10 @@ Proof.
   cbv [liftA2 Applicative__Seq Data.Sequence.Internal.Applicative__Seq_liftA2 liftA2__ liftA2Seq].
   destruct tb as [tb].
   pose proof (valid_viewl ta Hta) as HtaL.
-  pose proof (size_viewl ta) as Sta.
+  pose proof (size_viewl ta) as Sta; prove_assumptions_of Sta; auto.
   destruct (viewl ta) as [ | a ta' ]; [ constructor | ].
   pose proof (valid_viewr ta' HtaL) as HtaLR.
-  pose proof (size_viewr ta') as Sta'.
+  pose proof (size_viewr ta') as Sta'; prove_assumptions_of Sta'; auto.
   destruct (viewr ta') as [ | ta'' a'].
   { apply valid_fmap__Seq; assumption. }
   destruct ta'' as [ta''].
